@prefix : <http://matonto.org/ontologies/thermomechanics#> .
@prefix dl: <http://ontology.dumontierlab.com/> .
@prefix mat: <http://matonto.org/ontologies/matonto#> .
@prefix owl: <http://www.w3.org/2002/07/owl#> .
@prefix rdf: <http://www.w3.org/1999/02/22-rdf-syntax-ns#> .
@prefix xml: <http://www.w3.org/XML/1998/namespace> .
@prefix xsd: <http://www.w3.org/2001/XMLSchema#> .
@prefix rdfs: <http://www.w3.org/2000/01/rdf-schema#> .
@base <http://matonto.org/ontologies/thermomechanics> .

<http://matonto.org/ontologies/thermomechanics> rdf:type owl:Ontology ;
                                                
                                                owl:versionInfo "1.1" ;
                                                
                                                rdfs:comment "A materials science sub-domain ontology that encapsulates thermomechanics." ;
                                                
                                                owl:imports <http://matonto.org/ontologies/matonto> ;
                                                
                                                owl:versionIRI <http://matonto.org/ontologies/thermomechanics/1.1> .


#################################################################
#
#    Classes
#
#################################################################


###  http://matonto.org/ontologies/thermomechanics#BulkModulus

:BulkModulus rdf:type owl:Class ;
             
             rdfs:label "bulk modulus" ;
             
             rdfs:subClassOf :ElasticModulus ;
             
             mat:commonSymbol "K" ;
             
             rdfs:comment "The bulk modulus describes volumetric elasticity, or the tendency of an object to deform in all directions when uniformly loaded in all directions; it is defined as volumetric stress over volumetric strain, and is the inverse of compressibility. The bulk modulus is an extension of Young's modulus to three dimensions." .



###  http://matonto.org/ontologies/thermomechanics#ElasticModulus

:ElasticModulus rdf:type owl:Class ;
                
                rdfs:label "elastic modulus" ;
                
                rdfs:subClassOf dl:MeasuredProperty ,
                                [ rdf:type owl:Restriction ;
                                  owl:onProperty dl:hasUnit ;
                                  owl:allValuesFrom dl:PressureUnit
                                ] ,
                                [ rdf:type owl:Restriction ;
                                  owl:onProperty dl:hasUnit ;
                                  owl:someValuesFrom dl:PressureUnit
                                ] ;
                
                mat:commonSymbol "E" ;
                
                <http://www.w3.org/2004/02/skos/core#altLabel> "modulus of elasticity" ;
                
                rdfs:comment "An elastic modulus, or modulus of elasticity, is the mathematical description of an object or substance's tendency to be deformed elastically (i.e., non-permanently) when a force is applied to it. The elastic modulus of an object is defined as the slope of its stressâ€“strain curve in the elastic deformation region." .



###  http://matonto.org/ontologies/thermomechanics#FlexuralModulus

:FlexuralModulus rdf:type owl:Class ;
                 
                 rdfs:label "flexural modulus" ;
                 
                 rdfs:subClassOf mat:IntensiveProperty ,
                                 [ rdf:type owl:Restriction ;
                                   owl:onProperty dl:hasUnit ;
                                   owl:someValuesFrom dl:PressureUnit
                                 ] ,
                                 [ rdf:type owl:Restriction ;
                                   owl:onProperty dl:hasUnit ;
                                   owl:allValuesFrom dl:PressureUnit
                                 ] ;
                 
                 rdfs:comment "In mechanics, the flexural modulus or bending modulus is the ratio of stress to strain in flexural deformation, or the tendency for a material to bend. It is determined from the slope of a stress-strain curve produced by a flexural test, and uses units of force per area." ;
                 
                 <http://www.w3.org/2004/02/skos/core#altLabel> "bending modulus" ;
                 
                 mat:commonSymbol "E" .



###  http://matonto.org/ontologies/thermomechanics#FlexuralStrength

:FlexuralStrength rdf:type owl:Class ;
                  
                  rdfs:label "flexural strength" ;
                  
                  rdfs:subClassOf dl:MeasuredProperty ,
                                  [ rdf:type owl:Restriction ;
                                    owl:onProperty dl:hasUnit ;
                                    owl:someValuesFrom dl:PressureUnit
                                  ] ,
                                  [ rdf:type owl:Restriction ;
                                    owl:onProperty dl:hasUnit ;
                                    owl:allValuesFrom dl:PressureUnit
                                  ] ;
                  
                  <http://www.w3.org/2004/02/skos/core#altLabel> "modulus of rupture" ,
                                                                 "bend strength" ;
                  
                  rdfs:comment "Flexural strength is a mechanical parameter for brittle material, is defined as a material's ability to resist deformation under load." .



###  http://matonto.org/ontologies/thermomechanics#FractureToughness

:FractureToughness rdf:type owl:Class ;
                   
                   rdfs:label "fracture toughness" ;
                   
                   rdfs:subClassOf dl:MeasuredProperty ;
                   
                   mat:commonSymbol "K" .



###  http://matonto.org/ontologies/thermomechanics#GrainSize

:GrainSize rdf:type owl:Class ;
           
           rdfs:label "grain size" ;
           
           rdfs:subClassOf dl:MeasuredProperty ,
                           [ rdf:type owl:Restriction ;
                             owl:onProperty dl:hasUnit ;
                             owl:someValuesFrom dl:LengthUnit
                           ] ,
                           [ rdf:type owl:Restriction ;
                             owl:onProperty dl:hasUnit ;
                             owl:allValuesFrom dl:LengthUnit
                           ] ;
           
           <http://www.w3.org/2004/02/skos/core#altLabel> "particle size" ;
           
           rdfs:comment "Grain size refers to the diameter of individual grains of sediment, or the lithified particles in clastic rocks. The term may also be applied to other granular materials. This is different from the crystallite size, which is the size of a single crystal inside the particles or grains. A single grain can be composed of several crystals. Granular material can range from very small colloidal particles, through clay, silt, sand, and gravel, to boulders." .



###  http://matonto.org/ontologies/thermomechanics#ShearModulus

:ShearModulus rdf:type owl:Class ;
              
              rdfs:label "shear modulus" ;
              
              rdfs:subClassOf :ElasticModulus ;
              
              rdfs:comment "The shear modulus describes an object's tendency to shear (the deformation of shape at constant volume) when acted upon by opposing forces; it is defined as shear stress over shear strain. The shear modulus is part of the derivation of viscosity." ;
              
              mat:commonSymbol "G" ;
              
              <http://www.w3.org/2004/02/skos/core#altLabel> "modulus of rigidity" .



###  http://matonto.org/ontologies/thermomechanics#Stress

:Stress rdf:type owl:Class ;
        
        rdfs:subClassOf dl:MeasuredProperty ,
                        [ rdf:type owl:Restriction ;
                          owl:onProperty dl:hasUnit ;
                          owl:someValuesFrom dl:PressureUnit
                        ] ,
                        [ rdf:type owl:Restriction ;
                          owl:onProperty dl:hasUnit ;
                          owl:allValuesFrom dl:PressureUnit
                        ] ;
        
        rdfs:comment "In continuum mechanics, stress is a physical quantity that expresses the internal forces that neighbouring particles of a continuous material exert on each other." .



###  http://matonto.org/ontologies/thermomechanics#UltimateTensileStrength

:UltimateTensileStrength rdf:type owl:Class ;
                         
                         rdfs:label "ultimate tensile strength" ;
                         
                         rdfs:subClassOf dl:MeasuredProperty ,
                                         [ rdf:type owl:Restriction ;
                                           owl:onProperty dl:hasUnit ;
                                           owl:allValuesFrom dl:PressureUnit
                                         ] ,
                                         [ rdf:type owl:Restriction ;
                                           owl:onProperty dl:hasUnit ;
                                           owl:someValuesFrom dl:PressureUnit
                                         ] ;
                         
                         <http://www.w3.org/2004/02/skos/core#altLabel> "TS" ,
                                                                        "ultimate strength" ,
                                                                        "UTS" ;
                         
                         rdfs:comment "Ultimate tensile strength is the maximum stress that a material can withstand while being stretched or pulled before failing or breaking." ;
                         
                         <http://www.w3.org/2004/02/skos/core#altLabel> "tensile strength" .



###  http://matonto.org/ontologies/thermomechanics#WeibullModulus

:WeibullModulus rdf:type owl:Class ;
                
                rdfs:label "weibull modulus" ;
                
                rdfs:subClassOf dl:MeasuredProperty ;
                
                rdfs:comment "The Weibull modulus is a dimensionless parameter of the Weibull distribution which is used to describe variability in measured material strength of brittle materials." .



###  http://matonto.org/ontologies/thermomechanics#YoungsModulus

:YoungsModulus rdf:type owl:Class ;
               
               rdfs:label "youngs modulus" ;
               
               rdfs:subClassOf :ElasticModulus ;
               
               <http://www.w3.org/2004/02/skos/core#altLabel> "Young's modulus" ,
                                                              "tensile modulus" ;
               
               rdfs:comment "Young's modulus is a measure of the stiffness of an elastic isotropic material and is a quantity used to characterize materials. It is defined as the ratio of the stress along an axis over the strain along that axis in the range of stress in which Hooke's law holds." ;
               
               mat:commonSymbol "E" .





#################################################################
#
#    Individuals
#
#################################################################


###  http://matonto.org/ontologies/thermomechanics#unit_gigapascal

:unit_gigapascal rdf:type dl:PressureUnit ,
                          owl:NamedIndividual ;
                 
                 rdfs:label "gigapascal" ;
                 
                 dl:isScaledBy "1.0E9"^^xsd:double ;
                 
                 mat:symbol "GPa" ;
                 
                 dl:derivesFrom dl:unit_pascal .



###  http://matonto.org/ontologies/thermomechanics#unit_hectopascal

:unit_hectopascal rdf:type dl:PressureUnit ,
                           owl:NamedIndividual ;
                  
                  rdfs:label "hectopascal" ;
                  
                  dl:isScaledBy "100.0"^^xsd:double ;
                  
                  mat:symbol "hPa" ;
                  
                  dl:derivesFrom dl:unit_pascal .



###  http://matonto.org/ontologies/thermomechanics#unit_kilopascal

:unit_kilopascal rdf:type dl:PressureUnit ,
                          owl:NamedIndividual ;
                 
                 rdfs:label "kilopascal" ;
                 
                 dl:isScaledBy "1000.0"^^xsd:double ;
                 
                 mat:symbol "kPa" ;
                 
                 dl:derivesFrom dl:unit_pascal .



###  http://matonto.org/ontologies/thermomechanics#unit_megapascal

:unit_megapascal rdf:type dl:PressureUnit ,
                          owl:NamedIndividual ;
                 
                 rdfs:label "megapascal" ;
                 
                 dl:isScaledBy "1000000.0"^^xsd:double ;
                 
                 mat:symbol "MPa" ;
                 
                 dl:derivesFrom dl:unit_pascal .



###  http://matonto.org/ontologies/thermomechanics#unit_meter_sqrt

:unit_meter_sqrt rdf:type dl:Unit ,
                          owl:NamedIndividual ;
                 
                 rdfs:label "root meter" ;
                 
                 dl:isRaisedToPowerOf "0.5"^^xsd:double ;
                 
                 dl:derivesFrom dl:unit_meter .



###  http://matonto.org/ontologies/thermomechanics#unit_micrometer

:unit_micrometer rdf:type dl:LengthUnit ,
                          owl:NamedIndividual ;
                 
                 rdfs:label "micrometer" ;
                 
                 dl:isScaledBy "1.0E-6"^^xsd:double ;
                 
                 rdfs:comment "The micrometer is an SI derived unit of length equaling 1Ã—10âˆ’6 of a meter; that is, one millionth of a meter (or one thousandth of a millimeter, 0.001 mm, or about 0.000039 inch)." ;
                 
                 mat:symbol "Âµm" ;
                 
                 <http://www.w3.org/2004/02/skos/core#altLabel> "micrometre" ;
                 
                 dl:derivesFrom dl:unit_meter .



###  http://matonto.org/ontologies/thermomechanics#unit_pascal_1_meter_sqrt

:unit_pascal_1_meter_sqrt rdf:type dl:Unit ,
                                   owl:NamedIndividual ;
                          
                          rdfs:label "pascal root meter" ;
                          
                          rdfs:comment "Pa*m1/2 are the units for fracture toughness" ;
                          
                          dl:derivesFrom :unit_meter_sqrt ,
                                         dl:unit_pascal .



###  http://ontology.dumontierlab.com/unit_meter

dl:unit_meter <http://www.w3.org/2004/02/skos/core#altLabel> "metre" .




###  Generated by the OWL API (version 3.4.2) http://owlapi.sourceforge.net

